wip'

code/ecdsa/Hacl.Impl.EC.Core.fst
@@ -24,10 +24,14 @@ open Hacl.EC.Lemmas
 
 open FStar.Mul
 open Hacl.Impl.EC.MontgomeryLadder
+open Hacl.Impl.EC.ScalarMult.Radix
+
 open Spec.ECC.Curves
 
 
 #set-options "--z3rlimit 200 --max_fuel 0 --max_ifuel 0" 
+
+
 
 inline_for_extraction noextract 
 val toDomain_t: #c: curve -> value: felem c -> result: felem c -> Stack unit 
@@ -557,7 +561,7 @@ let uploadStartPointsS2P #c q result =
     lemma_pointAtInfInDomain #c x y z
 
 
-
+(* 
 inline_for_extraction noextract
 val secretToPublic_0: #c: curve -> #t: buftype -> q: point c -> result: point c -> 
   scalar: lbuffer_t t uint8 (getScalarLenBytes c) -> 
@@ -579,29 +583,25 @@ let secretToPublic_0 #c q result scalar tempBuffer =
   Hacl.Impl.EC.ScalarMult.Radix.montgomery_ladder_2_precomputed result scalar tempBuffer;
   copy q result
 
+ *)
 
 
-
-let secretToPublic_ml #c result scalar tempBuffer = 
+let secretToPublic #c #l result scalar tempBuffer = 
   let h0 = ST.get() in 
   let len = getCoordinateLenU64 c in 
   let q = sub tempBuffer (size 0) (size 3 *! len) in
   let buff = sub tempBuffer (size 3 *! len) (size 17 *! len) in 
-
-  secretToPublic_0 q result scalar buff;
-  norm q result buff
-
-
-let secretToPublic_radix #c result scalar tempBuffer = 
-  let h0 = ST.get() in 
-  let len = getCoordinateLenU64 c in 
-  let q = sub tempBuffer (size 0) (size 3 *! len) in
-  let buff = sub tempBuffer (size 3 *! len) (size 17 *! len) in 
-
-  secretToPublic_0 q result scalar buff;
-  norm q result buff
-
-
+  match l with 
+  |ML -> 
+    begin
+      secretToPublic_0 q result scalar buff;
+      norm q result buff
+    end
+  |Radix  -> 
+    begin
+      secretToPublic_0 q result scalar buff;
+      norm q result buff
+    end
 
 
 inline_for_extraction noextract
